Finish full crt and csr, extracting.

src/riot/x509/X509.BasicFields.Version.fst
@@ -16,8 +16,58 @@ let filter_x509_version
 : GTot bool
 = 0l <= x && x <= 2l
 
-let x509_version_t: Type
+let x509_version_payload_t: Type
 = parse_filter_refine filter_x509_version
+
+let parse_x509_version_payload
+: parser _ x509_version_payload_t
+= parse_asn1_TLV_of_type INTEGER
+  `parse_filter`
+  filter_x509_version
+
+let serialize_x509_version_payload
+: serializer parse_x509_version_payload
+= serialize_asn1_TLV_of_type INTEGER
+  `serialize_filter`
+  filter_x509_version
+
+let lemma_serialize_x509_version_payload_unfold
+  (x: x509_version_payload_t)
+= lemma_serialize_asn1_integer_TLV_unfold x
+
+let lemma_serialize_x509_version_payload_size
+  (x: x509_version_payload_t)
+= lemma_serialize_asn1_integer_TLV_size x
+
+let lemma_serialize_x509_version_payload_size_exact
+  (x: x509_version_payload_t)
+: Lemma (length_of_opaque_serialization serialize_x509_version_payload x == 3)
+= lemma_serialize_asn1_integer_TLV_size x;
+  assert (length_of_opaque_serialization serialize_x509_version_payload x == length_of_asn1_primitive_TLV #INTEGER x)
+
+let serialize32_x509_version_payload_backwards
+: serializer32_backwards serialize_x509_version_payload
+= serialize32_asn1_TLV_backwards_of_type INTEGER
+  `serialize32_filter_backwards`
+  filter_x509_version
+
+let length_of_x509_version_payload ()
+: GTot (l: asn1_value_length_of_type SEQUENCE
+           { forall (x: x509_version_payload_t). l == length_of_opaque_serialization serialize_x509_version_payload x })
+= Classical.forall_intro lemma_serialize_x509_version_payload_size_exact;
+  3
+
+let len_of_x509_version_payload ()
+: Tot (len: asn1_value_int32_of_type SEQUENCE
+           { forall (x: x509_version_payload_t). v len == length_of_opaque_serialization serialize_x509_version_payload x })
+= Classical.forall_intro lemma_serialize_x509_version_payload_size_exact;
+  3ul
+
+
+let x509_version_t: Type
+= CUSTOM_TAG CONTEXT_SPECIFIC CONSTRUCTED 0uy
+  `inbound_envelop_tag_with_value_of`
+  serialize_x509_version_payload
 
 let x509_version_1: x509_version_t = 0l
 let x509_version_2: x509_version_t = 1l
@@ -25,44 +75,79 @@ let x509_version_3: x509_version_t = 2l
 
 let parse_x509_version
 : parser _ x509_version_t
-= parse_asn1_TLV_of_type INTEGER
-  `parse_filter`
-  filter_x509_version
+= CUSTOM_TAG CONTEXT_SPECIFIC CONSTRUCTED 0uy
+  `parse_asn1_envelop_tag_with_TLV`
+  serialize_x509_version_payload
 
 let serialize_x509_version
 : serializer parse_x509_version
-= serialize_asn1_TLV_of_type INTEGER
-  `serialize_filter`
-  filter_x509_version
+= CUSTOM_TAG CONTEXT_SPECIFIC CONSTRUCTED 0uy
+  `serialize_asn1_envelop_tag_with_TLV`
+  serialize_x509_version_payload
 
 let lemma_serialize_x509_version_unfold
   (x: x509_version_t)
-= lemma_serialize_asn1_integer_TLV_unfold x
+: Lemma (
+  predicate_serialize_asn1_envelop_tag_with_TLV_unfold
+    (CUSTOM_TAG CONTEXT_SPECIFIC CONSTRUCTED 0uy)
+    (serialize_x509_version_payload)
+    (x)
+)
+= lemma_serialize_asn1_envelop_tag_with_TLV_unfold
+    (CUSTOM_TAG CONTEXT_SPECIFIC CONSTRUCTED 0uy)
+    (serialize_x509_version_payload)
+    (x)
 
 let lemma_serialize_x509_version_size
   (x: x509_version_t)
-= lemma_serialize_asn1_integer_TLV_size x
+: Lemma (
+  predicate_serialize_asn1_envelop_tag_with_TLV_size
+    (CUSTOM_TAG CONTEXT_SPECIFIC CONSTRUCTED 0uy)
+    (serialize_x509_version_payload)
+    (x)
+)
+= lemma_serialize_asn1_envelop_tag_with_TLV_size
+    (CUSTOM_TAG CONTEXT_SPECIFIC CONSTRUCTED 0uy)
+    (serialize_x509_version_payload)
+    (x)
 
 let lemma_serialize_x509_version_size_exact
   (x: x509_version_t)
-: Lemma (length_of_opaque_serialization serialize_x509_version x == 3)
-= lemma_serialize_asn1_integer_TLV_size x;
-  assert (length_of_opaque_serialization serialize_x509_version x == length_of_asn1_primitive_TLV #INTEGER x)
-
-let serialize32_x509_version_backwards
-: serializer32_backwards serialize_x509_version
-= serialize32_asn1_TLV_backwards_of_type INTEGER
-  `serialize32_filter_backwards`
-  filter_x509_version
+: Lemma (
+  length_of_opaque_serialization serialize_x509_version x ==
+  5
+)
+= lemma_serialize_x509_version_size x;
+  lemma_serialize_x509_version_payload_size_exact x
 
 let length_of_x509_version ()
 : GTot (l: asn1_value_length_of_type SEQUENCE
-           { forall (x: x509_version_t). l == length_of_opaque_serialization serialize_x509_version x })
+           { forall (x: x509_version_t).
+               let _ = lemma_serialize_x509_version_size_exact x in
+               l == length_of_opaque_serialization serialize_x509_version x })
 = Classical.forall_intro lemma_serialize_x509_version_size_exact;
-  3
+  5
 
 let len_of_x509_version ()
 : Tot (len: asn1_value_int32_of_type SEQUENCE
-           { forall (x: x509_version_t). v len == length_of_opaque_serialization serialize_x509_version x })
+           { forall (x: x509_version_t).
+               let _ = lemma_serialize_x509_version_size_exact x in
+               v len == length_of_opaque_serialization serialize_x509_version x })
 = Classical.forall_intro lemma_serialize_x509_version_size_exact;
-  3ul
+  5ul
+
+let serialize32_x509_version_backwards
+: serializer32_backwards serialize_x509_version
+= CUSTOM_TAG CONTEXT_SPECIFIC CONSTRUCTED 0uy
+  `serialize32_asn1_envelop_tag_with_TLV_backwards`
+  serialize32_x509_version_payload_backwards
+
+let x509_get_version
+  (x: x509_version_payload_t)
+: Tot (x509_version_t)
+= x
+
+let s =
+  serialize_x509_version
+  `serialize_nondep_then`
+  serialize_x509_version
