src/riot/RIoT.X509.AliasKeyTBS.Extensions.AuthKeyIdentifier.fst
@@ -1,0 +1,297 @@
+module RIoT.X509.AliasKeyTBS.Extensions.AuthKeyIdentifier
+
+open ASN1.Spec
+open ASN1.Low
+open X509
+open X509.BasicFields.Extension2
+open FStar.Integers
+
+module B32 = FStar.Bytes
+
+#set-options "--z3rlimit 64 --fuel 0 --ifuel 0"
+
+(* extValue payload *)
+
+let aliasKeyTBS_extensions_authKeyID_extValue_payload_t: Type0
+= x509_authKeyID_keyIdentifier_t
+
+let parse_aliasKeyTBS_extensions_authKeyID_extValue_payload
+: parser _ aliasKeyTBS_extensions_authKeyID_extValue_payload_t
+= parse_x509_authKeyID_keyIdentifier
+
+let serialize_aliasKeyTBS_extensions_authKeyID_extValue_payload
+: serializer parse_aliasKeyTBS_extensions_authKeyID_extValue_payload
+= serialize_x509_authKeyID_keyIdentifier
+
+let serialize32_aliasKeyTBS_extensions_authKeyID_extValue_payload_backwards
+: serializer32_backwards serialize_aliasKeyTBS_extensions_authKeyID_extValue_payload
+= serialize32_x509_authKeyID_keyIdentifier_backwards
+
+let lemma_serialize_aliasKeyTBS_extensions_authKeyID_extValue_payload_unfold
+  (x: aliasKeyTBS_extensions_authKeyID_extValue_payload_t)
+: Lemma (
+  serialize_aliasKeyTBS_extensions_authKeyID_extValue_payload `serialize` x ==
+  serialize_x509_authKeyID_keyIdentifier `serialize` x
+)
+= ()
+
+let length_of_aliasKeyTBS_extensions_authKeyID_extValue_payload
+  (keyID: datatype_of_asn1_type OCTET_STRING
+          { valid_authKeyID_keyIdentifier_ingredients keyID })
+: GTot (nat)
+= length_of_x509_authKeyID_keyIdentifier keyID
+
+let valid_aliasKeyTBS_extensions_authKeyID_extValue_payload_ingredients
+  (keyID: datatype_of_asn1_type OCTET_STRING)
+: Type0
+= valid_authKeyID_keyIdentifier_ingredients keyID /\
+  length_of_aliasKeyTBS_extensions_authKeyID_extValue_payload keyID
+  <= asn1_value_length_max_of_type SEQUENCE
+
+let len_of_aliasKeyTBS_extensions_authKeyID_extValue_payload
+  (keyID: datatype_of_asn1_type OCTET_STRING
+          { valid_aliasKeyTBS_extensions_authKeyID_extValue_payload_ingredients keyID })
+: Tot (len: asn1_value_int32_of_type SEQUENCE
+            { v len == length_of_aliasKeyTBS_extensions_authKeyID_extValue_payload keyID })
+= len_of_x509_authKeyID_keyIdentifier keyID
+
+let lemma_serialize_aliasKeyTBS_extensions_authKeyID_extValue_payload_size
+  (x: aliasKeyTBS_extensions_authKeyID_extValue_payload_t
+      { valid_aliasKeyTBS_extensions_authKeyID_extValue_payload_ingredients x })
+: Lemma (
+  length_of_opaque_serialization serialize_aliasKeyTBS_extensions_authKeyID_extValue_payload x ==
+  length_of_opaque_serialization serialize_x509_authKeyID_keyIdentifier x /\
+  length_of_opaque_serialization serialize_aliasKeyTBS_extensions_authKeyID_extValue_payload x ==
+  length_of_aliasKeyTBS_extensions_authKeyID_extValue_payload x
+)
+= lemma_serialize_aliasKeyTBS_extensions_authKeyID_extValue_payload_unfold x;
+  lemma_serialize_x509_authKeyID_keyIdentifier_size_exact x
+
+(* extValue *)
+
+let aliasKeyTBS_extensions_authKeyID_extValue_t
+= inbound_sequence_value_of
+  (**) (serialize_aliasKeyTBS_extensions_authKeyID_extValue_payload)
+
+let parse_aliasKeyTBS_extensions_authKeyID_extValue
+: parser (parse_asn1_envelop_tag_with_TLV_kind SEQUENCE) aliasKeyTBS_extensions_authKeyID_extValue_t
+= aliasKeyTBS_extensions_authKeyID_extValue_t
+  `coerce_parser`
+  parse_asn1_sequence_TLV
+  (**) (serialize_aliasKeyTBS_extensions_authKeyID_extValue_payload)
+
+let serialize_aliasKeyTBS_extensions_authKeyID_extValue
+: serializer parse_aliasKeyTBS_extensions_authKeyID_extValue
+= coerce_parser_serializer
+    (parse_aliasKeyTBS_extensions_authKeyID_extValue)
+    (serialize_asn1_sequence_TLV
+    (**) (serialize_aliasKeyTBS_extensions_authKeyID_extValue_payload))
+    ()
+
+let serialize32_aliasKeyTBS_extensions_authKeyID_extValue_backwards
+: serializer32_backwards serialize_aliasKeyTBS_extensions_authKeyID_extValue
+= coerce_serializer32_backwards
+    (serialize_aliasKeyTBS_extensions_authKeyID_extValue)
+    (serialize32_asn1_sequence_TLV_backwards
+    (**) (serialize32_aliasKeyTBS_extensions_authKeyID_extValue_payload_backwards))
+    ()
+
+let lemma_serialize_aliasKeyTBS_extensions_authKeyID_extValue_unfold
+  (x: aliasKeyTBS_extensions_authKeyID_extValue_t)
+: Lemma (
+  predicate_serialize_asn1_sequence_TLV_unfold
+    (serialize_aliasKeyTBS_extensions_authKeyID_extValue_payload)
+    (x)
+)
+= lemma_serialize_asn1_sequence_TLV_unfold
+    (serialize_aliasKeyTBS_extensions_authKeyID_extValue_payload)
+    (x)
+
+let lemma_serialize_aliasKeyTBS_extensions_authKeyID_extValue_size
+  (x: aliasKeyTBS_extensions_authKeyID_extValue_t)
+: Lemma (
+  predicate_serialize_asn1_sequence_TLV_size
+    (serialize_aliasKeyTBS_extensions_authKeyID_extValue_payload)
+    (x)
+)
+= lemma_serialize_asn1_sequence_TLV_size
+    (serialize_aliasKeyTBS_extensions_authKeyID_extValue_payload)
+    (x)
+
+let valid_aliasKeyTBS_extensions_authKeyID_extValue_ingredients
+  (keyID: datatype_of_asn1_type OCTET_STRING)
+= valid_aliasKeyTBS_extensions_authKeyID_extValue_payload_ingredients keyID /\
+  length_of_TLV
+    (SEQUENCE)
+    (length_of_aliasKeyTBS_extensions_authKeyID_extValue_payload keyID)
+  <= asn1_value_length_max_of_type OCTET_STRING
+
+let length_of_aliasKeyTBS_extensions_authKeyID_extValue
+  (keyID: datatype_of_asn1_type OCTET_STRING
+          { valid_aliasKeyTBS_extensions_authKeyID_extValue_ingredients keyID })
+: GTot (asn1_value_length_of_type OCTET_STRING)
+= length_of_TLV
+    (SEQUENCE)
+    (length_of_aliasKeyTBS_extensions_authKeyID_extValue_payload keyID)
+
+let len_of_aliasKeyTBS_extensions_authKeyID_extValue
+  (keyID: datatype_of_asn1_type OCTET_STRING
+          { valid_aliasKeyTBS_extensions_authKeyID_extValue_ingredients keyID })
+: Tot (len: asn1_value_int32_of_type OCTET_STRING
+            { v len == length_of_aliasKeyTBS_extensions_authKeyID_extValue keyID })
+= len_of_TLV
+    (SEQUENCE)
+    (len_of_aliasKeyTBS_extensions_authKeyID_extValue_payload keyID)
+
+let lemma_serialize_aliasKeyTBS_extensions_authKeyID_extValue_size_exact
+  (x: aliasKeyTBS_extensions_authKeyID_extValue_t
+      { valid_aliasKeyTBS_extensions_authKeyID_extValue_ingredients x })
+: Lemma (
+  length_of_opaque_serialization serialize_aliasKeyTBS_extensions_authKeyID_extValue x ==
+  length_of_aliasKeyTBS_extensions_authKeyID_extValue x
+)
+= lemma_serialize_aliasKeyTBS_extensions_authKeyID_extValue_size x;
+    lemma_serialize_aliasKeyTBS_extensions_authKeyID_extValue_payload_size x
+
+let x509_get_aliasKeyTBS_extensions_authKeyID_extValue
+  (keyID: datatype_of_asn1_type OCTET_STRING
+          { valid_aliasKeyTBS_extensions_authKeyID_extValue_ingredients keyID })
+: Tot (aliasKeyTBS_extensions_authKeyID_extValue_t)
+= (* Prf *) Classical.forall_intro lemma_serialize_x509_authKeyID_keyIdentifier_size_exact;
+  x509_get_authKeyID_keyIdentifier keyID
+
+(* ext *)
+
+let aliasKeyTBS_extensions_authKeyID_t: Type
+= x509_extension_t
+  (**) (OID_AUTHORITY_KEY_IDENTIFIER)
+  (**) (serialize_aliasKeyTBS_extensions_authKeyID_extValue)
+
+let parse_aliasKeyTBS_extensions_authKeyID
+// : parser _ aliasKeyTBS_extensions_authKeyID_t
+= aliasKeyTBS_extensions_authKeyID_t
+  `coerce_parser`
+  parse_x509_extension
+  (**) (OID_AUTHORITY_KEY_IDENTIFIER)
+  (**) (serialize_aliasKeyTBS_extensions_authKeyID_extValue)
+
+let serialize_aliasKeyTBS_extensions_authKeyID
+: serializer parse_aliasKeyTBS_extensions_authKeyID
+= coerce_parser_serializer
+    (parse_aliasKeyTBS_extensions_authKeyID)
+    (serialize_x509_extension
+    (**) (OID_AUTHORITY_KEY_IDENTIFIER)
+    (**) (serialize_aliasKeyTBS_extensions_authKeyID_extValue))
+    ()
+
+noextract inline_for_extraction
+let serialize32_aliasKeyTBS_extensions_authKeyID_backwards
+: serializer32_backwards serialize_aliasKeyTBS_extensions_authKeyID
+= coerce_serializer32_backwards
+    (serialize_aliasKeyTBS_extensions_authKeyID)
+    (serialize32_x509_extension_backwards
+    (**) (OID_AUTHORITY_KEY_IDENTIFIER)
+    (**) (serialize32_aliasKeyTBS_extensions_authKeyID_extValue_backwards))
+    ()
+
+let lemma_serialize_aliasKeyTBS_extensions_authKeyID_unfold
+  (x: aliasKeyTBS_extensions_authKeyID_t)
+: Lemma (
+  predicate_serialize_x509_extension_unfold
+    (**) (OID_AUTHORITY_KEY_IDENTIFIER)
+    (**) (serialize_aliasKeyTBS_extensions_authKeyID_extValue)
+    (**) (x)
+)
+= lemma_serialize_x509_extension_unfold
+    (**) (OID_AUTHORITY_KEY_IDENTIFIER)
+    (**) (serialize_aliasKeyTBS_extensions_authKeyID_extValue)
+    (**) (x)
+
+let lemma_serialize_aliasKeyTBS_extensions_authKeyID_size
+  (x: aliasKeyTBS_extensions_authKeyID_t)
+: Lemma (
+  predicate_serialize_x509_extension_size
+    (**) (OID_AUTHORITY_KEY_IDENTIFIER)
+    (**) (serialize_aliasKeyTBS_extensions_authKeyID_extValue)
+    (**) (x)
+)
+= lemma_serialize_x509_extension_size
+    (**) (OID_AUTHORITY_KEY_IDENTIFIER)
+    (**) (serialize_aliasKeyTBS_extensions_authKeyID_extValue)
+    (**) (x)
+
+let valid_aliasKeyTBS_extensions_authKeyID_ingredients
+  (keyID: datatype_of_asn1_type OCTET_STRING)
+: Type0
+= valid_aliasKeyTBS_extensions_authKeyID_extValue_ingredients keyID /\
+  (let _ = lemma_serialize_aliasKeyTBS_extensions_authKeyID_extValue_payload_size keyID;
+           lemma_serialize_aliasKeyTBS_extensions_authKeyID_extValue_size_exact (x509_get_aliasKeyTBS_extensions_authKeyID_extValue keyID) in
+   length_of_x509_extension_payload_unbounded
+     (OID_AUTHORITY_KEY_IDENTIFIER)
+     (serialize_aliasKeyTBS_extensions_authKeyID_extValue)
+     (x509_get_aliasKeyTBS_extensions_authKeyID_extValue keyID)
+     (length_of_aliasKeyTBS_extensions_authKeyID_extValue (x509_get_aliasKeyTBS_extensions_authKeyID_extValue keyID))
+   <= asn1_value_length_max_of_type (SEQUENCE))
+
+let length_of_aliasKeyTBS_extensions_authKeyID
+  (keyID: datatype_of_asn1_type OCTET_STRING
+          { valid_aliasKeyTBS_extensions_authKeyID_ingredients keyID })
+: GTot (asn1_TLV_length_of_type SEQUENCE)
+= lemma_serialize_aliasKeyTBS_extensions_authKeyID_extValue_payload_size keyID;
+  lemma_serialize_aliasKeyTBS_extensions_authKeyID_extValue_size_exact (x509_get_aliasKeyTBS_extensions_authKeyID_extValue keyID);
+  length_of_x509_extension
+    (OID_AUTHORITY_KEY_IDENTIFIER)
+    (serialize_aliasKeyTBS_extensions_authKeyID_extValue)
+    (x509_get_aliasKeyTBS_extensions_authKeyID_extValue keyID)
+    (length_of_aliasKeyTBS_extensions_authKeyID_extValue (x509_get_aliasKeyTBS_extensions_authKeyID_extValue keyID))
+
+let len_of_aliasKeyTBS_extensions_authKeyID
+  (keyID: datatype_of_asn1_type OCTET_STRING
+          { valid_aliasKeyTBS_extensions_authKeyID_ingredients keyID })
+: Tot (len: asn1_TLV_int32_of_type SEQUENCE
+            { v len == length_of_aliasKeyTBS_extensions_authKeyID keyID })
+= lemma_serialize_aliasKeyTBS_extensions_authKeyID_extValue_payload_size keyID;
+  lemma_serialize_aliasKeyTBS_extensions_authKeyID_extValue_size_exact (x509_get_aliasKeyTBS_extensions_authKeyID_extValue keyID);
+  len_of_x509_extension
+    (OID_AUTHORITY_KEY_IDENTIFIER)
+    (Ghost.hide serialize_aliasKeyTBS_extensions_authKeyID_extValue)
+    (x509_get_aliasKeyTBS_extensions_authKeyID_extValue keyID)
+    (len_of_aliasKeyTBS_extensions_authKeyID_extValue (x509_get_aliasKeyTBS_extensions_authKeyID_extValue keyID))
+
+let lemma_serialize_aliasKeyTBS_extensions_authKeyID_size_exact
+  (ext: aliasKeyTBS_extensions_authKeyID_t
+        { valid_aliasKeyTBS_extensions_authKeyID_ingredients (snd ext) })
+: Lemma (
+  length_of_opaque_serialization serialize_aliasKeyTBS_extensions_authKeyID ext ==
+  length_of_aliasKeyTBS_extensions_authKeyID (snd ext)
+)
+= lemma_serialize_aliasKeyTBS_extensions_authKeyID_extValue_size_exact (snd ext);
+  lemma_serialize_aliasKeyTBS_extensions_authKeyID_extValue_payload_size (snd ext <: aliasKeyTBS_extensions_authKeyID_extValue_t);
+  lemma_serialize_x509_extension_size_exact
+    (OID_AUTHORITY_KEY_IDENTIFIER)
+    (serialize_aliasKeyTBS_extensions_authKeyID_extValue)
+    (ext)
+    (length_of_aliasKeyTBS_extensions_authKeyID_extValue (snd ext))
+
+let x509_get_aliasKeyTBS_extensions_authKeyID
+  (criticality: datatype_of_asn1_type BOOLEAN)
+  (keyID: datatype_of_asn1_type OCTET_STRING
+          { valid_aliasKeyTBS_extensions_authKeyID_ingredients keyID })
+: Tot (aliasKeyTBS_extensions_authKeyID_t)
+= let extValue_payload: aliasKeyTBS_extensions_authKeyID_extValue_payload_t = keyID in
+  (* Prf *) lemma_serialize_aliasKeyTBS_extensions_authKeyID_extValue_payload_size extValue_payload;
+
+  let extValue: aliasKeyTBS_extensions_authKeyID_extValue_t = extValue_payload in
+  (* Prf *) lemma_serialize_aliasKeyTBS_extensions_authKeyID_extValue_size_exact extValue;
+
+  let ext: aliasKeyTBS_extensions_authKeyID_t = aliasKeyTBS_extensions_authKeyID_t
+                                     `coerce`
+                                     x509_get_extension
+                                       (OID_AUTHORITY_KEY_IDENTIFIER)
+                                       (serialize_aliasKeyTBS_extensions_authKeyID_extValue)
+                                       (extValue)
+                                       (len_of_aliasKeyTBS_extensions_authKeyID_extValue keyID)
+                                       (criticality)
+                                       in
+
+(* return *) ext
