src/riot/RIoT.X509.AliasKeyTBS.Extensions.BasicConstraints.fst
@@ -1,0 +1,64 @@
+module RIoT.X509.AliasKeyTBS.Extensions.BasicConstraints
+
+open ASN1.Spec
+open ASN1.Low
+open X509
+open FStar.Integers
+
+module B32 = FStar.Bytes
+
+#set-options "--z3rlimit 64 --fuel 0 --ifuel 0"
+
+noextract inline_for_extraction
+let aliasKeyTBS_extensions_basicConstraints_isCA: bool = false
+
+let aliasKeyTBS_extensions_basicConstraints_t: Type
+= x509_basicConstraints_t aliasKeyTBS_extensions_basicConstraints_isCA
+
+noextract inline_for_extraction
+let parse_aliasKeyTBS_extensions_basicConstraints
+// : parser parse_x509_extension_kind aliasKeyTBS_extensions_basicConstraints_t
+= aliasKeyTBS_extensions_basicConstraints_t
+  `coerce_parser`
+  parse_x509_basicConstraints aliasKeyTBS_extensions_basicConstraints_isCA
+
+let serialize_aliasKeyTBS_extensions_basicConstraints
+: serializer parse_aliasKeyTBS_extensions_basicConstraints
+= coerce_parser_serializer
+    (parse_aliasKeyTBS_extensions_basicConstraints)
+    (serialize_x509_basicConstraints aliasKeyTBS_extensions_basicConstraints_isCA)
+    ()
+
+noextract inline_for_extraction
+let serialize32_aliasKeyTBS_extensions_basicConstraints_backwards
+: serializer32_backwards serialize_aliasKeyTBS_extensions_basicConstraints
+= coerce_serializer32_backwards
+    (serialize_aliasKeyTBS_extensions_basicConstraints)
+    (serialize32_x509_basicConstraints_backwards aliasKeyTBS_extensions_basicConstraints_isCA)
+    ()
+
+let length_of_aliasKeyTBS_extensions_basicConstraints ()
+: GTot (asn1_TLV_length_of_type SEQUENCE)
+= length_of_x509_basicConstraints aliasKeyTBS_extensions_basicConstraints_isCA
+
+let len_of_aliasKeyTBS_extensions_basicConstraints ()
+: Tot (len: asn1_TLV_int32_of_type SEQUENCE
+            { v len == length_of_aliasKeyTBS_extensions_basicConstraints () })
+= len_of_x509_basicConstraints aliasKeyTBS_extensions_basicConstraints_isCA
+
+let lemma_serialize_aliasKeyTBS_extensions_basicConstraints_size_exact
+  (x: aliasKeyTBS_extensions_basicConstraints_t)
+: Lemma (
+  length_of_opaque_serialization serialize_aliasKeyTBS_extensions_basicConstraints x
+  == length_of_aliasKeyTBS_extensions_basicConstraints ()
+)
+= lemma_serialize_x509_basicConstraints_size_exact
+    (aliasKeyTBS_extensions_basicConstraints_isCA)
+    (x)
+
+let x509_get_aliasKeyTBS_extensions_basicConstraints
+  (criticality: datatype_of_asn1_type BOOLEAN)
+: Tot (aliasKeyTBS_extensions_basicConstraints_t)
+= x509_get_basicConstraints_isNotCA
+    (aliasKeyTBS_extensions_basicConstraints_isCA)
+    (criticality)
