src/riot/RIoT.X509.AliasKeyTBS.Extensions.ExtendedKeyUsage.fst
@@ -1,0 +1,102 @@
+module RIoT.X509.AliasKeyTBS.Extensions.ExtendedKeyUsage
+
+open ASN1.Spec
+open ASN1.Low
+open X509
+open FStar.Integers
+
+module B32 = FStar.Bytes
+module T = FStar.Tactics
+module P = FStar.Pervasives
+
+(* 4 fuels for the recursively defined 3-oid extendedKeyUsage *)
+#set-options "--z3rlimit 64 --fuel 4 --ifuel 0"
+
+noextract inline_for_extraction
+let aliasKeyCrt_extendedKeyUsage_oids
+: l: keyPurposeIDs_oids_t
+     { valid_x509_ext_key_usage_ingredients l }
+= [@inline_let]
+  let l = [OID_AT_CN; OID_AT_COUNTRY; OID_AT_ORGANIZATION] in
+  assert_norm (  valid_keyPurposeIDs l  );
+  // lemma_serialize_x509_keyPurposeIDs_size_norm l;
+  lemma_serialize_x509_keyPurposeIDs_size l;
+  l
+
+[@@T.postprocess_with (postprocess_x509_keyPurposeIDs (`%aliasKeyCrt_extendedKeyUsage_oids))]
+let aliasKeyTBS_extensions_extendedKeyUsage_t: Type
+= x509_ext_key_usage_t aliasKeyCrt_extendedKeyUsage_oids
+
+let lemma_aliasKeyTBS_extensions_extendedKeyUsage_norm ()
+: Lemma (
+  aliasKeyTBS_extensions_extendedKeyUsage_t == x509_ext_key_usage_t aliasKeyCrt_extendedKeyUsage_oids
+)
+= P.norm_spec
+    (norm_steps_x509_keyPurposeIDs (`%aliasKeyCrt_extendedKeyUsage_oids))
+    (x509_ext_key_usage_t aliasKeyCrt_extendedKeyUsage_oids)
+  // assert ( aliasKeyTBS_extensions_extendedKeyUsage_t == x509_ext_key_usage_t aliasKeyCrt_extendedKeyUsage_oids )
+  // by ( postprocess_x509_keyPurposeIDs (`%aliasKeyCrt_extendedKeyUsage_oids) () )
+
+let parse_aliasKeyTBS_extensions_extendedKeyUsage
+: parser X509.BasicFields.Extension2.parse_x509_extension_kind aliasKeyTBS_extensions_extendedKeyUsage_t
+= lemma_aliasKeyTBS_extensions_extendedKeyUsage_norm ();
+  aliasKeyTBS_extensions_extendedKeyUsage_t
+  `coerce_parser`
+  parse_x509_ext_key_usage aliasKeyCrt_extendedKeyUsage_oids
+
+let serialize_aliasKeyTBS_extensions_extendedKeyUsage
+: serializer parse_aliasKeyTBS_extensions_extendedKeyUsage
+= coerce_parser_serializer
+    (parse_aliasKeyTBS_extensions_extendedKeyUsage)
+    (serialize_x509_ext_key_usage aliasKeyCrt_extendedKeyUsage_oids)
+    (lemma_aliasKeyTBS_extensions_extendedKeyUsage_norm ())
+
+[@@T.postprocess_with (postprocess_x509_keyPurposeIDs (`%aliasKeyCrt_extendedKeyUsage_oids))]
+let serialize32_aliasKeyTBS_extensions_extendedKeyUsage_backwards
+: serializer32_backwards serialize_aliasKeyTBS_extensions_extendedKeyUsage
+= coerce_serializer32_backwards
+    (serialize_aliasKeyTBS_extensions_extendedKeyUsage)
+    (serialize32_x509_ext_key_usage_backwards aliasKeyCrt_extendedKeyUsage_oids)
+    (lemma_aliasKeyTBS_extensions_extendedKeyUsage_norm ())
+
+#push-options "--z3rlimit 256"
+let length_of_aliasKeyTBS_extensions_extendedKeyUsage ()
+: GTot (l: asn1_TLV_length_of_type SEQUENCE
+           { l == 29 })
+= length_of_x509_ext_key_usage aliasKeyCrt_extendedKeyUsage_oids
+#pop-options
+
+[@@T.postprocess_with (postprocess_x509_keyPurposeIDs (`%aliasKeyCrt_extendedKeyUsage_oids))]
+let len_of_aliasKeyTBS_extensions_extendedKeyUsage ()
+: Tot (len: asn1_TLV_int32_of_type SEQUENCE
+            { v len == length_of_aliasKeyTBS_extensions_extendedKeyUsage () })
+// (* FIXME: *) = len_of_x509_ext_key_usage aliasKeyCrt_extendedKeyUsage_oids
+= 29ul
+
+let lemma_serialize_aliasKeyTBS_extensions_extendedKeyUsage_size_exact
+  (x: aliasKeyTBS_extensions_extendedKeyUsage_t)
+: Lemma (
+  lemma_aliasKeyTBS_extensions_extendedKeyUsage_norm ();
+  length_of_opaque_serialization
+    serialize_aliasKeyTBS_extensions_extendedKeyUsage
+    x ==
+  length_of_aliasKeyTBS_extensions_extendedKeyUsage ()
+)
+= lemma_aliasKeyTBS_extensions_extendedKeyUsage_norm ();
+  lemma_x509_keyPurposeIDs_unique aliasKeyCrt_extendedKeyUsage_oids;
+  lemma_serialize_x509_ext_key_usage_size_exact
+    (aliasKeyCrt_extendedKeyUsage_oids)
+    (x509_ext_key_usage_t aliasKeyCrt_extendedKeyUsage_oids
+     `coerce`
+     x)
+
+[@@T.postprocess_with (postprocess_x509_keyPurposeIDs (`%aliasKeyCrt_extendedKeyUsage_oids))]
+let x509_get_aliasKeyTBS_extensions_extendedKeyUsage
+  (criticality: datatype_of_asn1_type BOOLEAN)
+: Tot (aliasKeyTBS_extensions_extendedKeyUsage_t)
+= lemma_aliasKeyTBS_extensions_extendedKeyUsage_norm ();
+  aliasKeyTBS_extensions_extendedKeyUsage_t
+  `coerce`
+  x509_get_ext_extendedKeyUsage
+    aliasKeyCrt_extendedKeyUsage_oids
+    criticality
