src/riot/RIoT.X509.AliasKeyTBS.fst
@@ -129,7 +129,8 @@ let parse_aliasKeyTBS_payload
 
 let serialize_aliasKeyTBS_payload
 : serializer (parse_aliasKeyTBS_payload)
-= serialize_synth
+=
+  serialize_synth
   (* p1 *) (parse_x509_version
             `nondep_then`
             parse_x509_serialNumber
@@ -160,7 +161,9 @@ let serialize_aliasKeyTBS_payload
             `serialize_nondep_then`
             serialize_subjectPublicKeyInfo
             `serialize_nondep_then`
-            serialize_x509_extensions_TLV serialize_aliasKeyTBS_extensions)
+            serialize_x509_extensions_TLV serialize_aliasKeyTBS_extensions
+            `coerce_parser_serializer _`
+            ())
   (* g1 *) (synth_aliasKeyTBS_payload_t')
   (* prf*) ()
 
@@ -184,8 +187,7 @@ let lemma_serialize_aliasKeyTBS_payload_unfold
   `Seq.append`
  (serialize_x509_extensions_TLV serialize_aliasKeyTBS_extensions `serialize` x.aliasKeyTBS_extensions)
 )
-=
-  serialize_nondep_then_eq
+= serialize_nondep_then_eq
   (* s1 *) (serialize_x509_version)
   (* s2 *) (serialize_x509_serialNumber)
   (* in *) (fst (fst (fst(fst (fst (fst (synth_aliasKeyTBS_payload_t' x)))))));
@@ -293,10 +295,37 @@ let lemma_serialize_aliasKeyTBS_payload_unfold
             `serialize_nondep_then`
             serialize_subjectPublicKeyInfo
             `serialize_nondep_then`
-            serialize_x509_extensions_TLV serialize_aliasKeyTBS_extensions)
+            serialize_x509_extensions_TLV serialize_aliasKeyTBS_extensions
+            `coerce_parser_serializer _`
+            ())
   (* g1 *) (synth_aliasKeyTBS_payload_t')
   (* prf*) ()
   (* in *) (x)
+
+let valid_aliasKeyTBS_ingredients
+  (serialNumber: x509_serialNumber_t)
+  (i_common:  x509_RDN_x520_attribute_string_t COMMON_NAME  IA5_STRING)
+  (i_org:     x509_RDN_x520_attribute_string_t ORGANIZATION IA5_STRING)
+  (i_country: x509_RDN_x520_attribute_string_t COUNTRY      PRINTABLE_STRING)
+  (s_common:  x509_RDN_x520_attribute_string_t COMMON_NAME  IA5_STRING)
+  (s_org:     x509_RDN_x520_attribute_string_t ORGANIZATION IA5_STRING)
+  (s_country: x509_RDN_x520_attribute_string_t COUNTRY      PRINTABLE_STRING)
+  (ku: key_usage_payload_t)
+  (keyID: datatype_of_asn1_type OCTET_STRING)
+  (version: datatype_of_asn1_type INTEGER)
+: Type0
+= valid_aliasKeyTBS_extensions_ingredients ku keyID version /\
+  length_of_aliasKeyTBS_extensions ku keyID version
+  <= asn1_value_length_max_of_type x509_extensions_outmost_explicit_tag /\
+  length_of_x509_version () +
+  length_of_x509_serialNumber serialNumber +
+  length_of_algorithmIdentifier () +
+  length_of_aliasKeyTBS_issuer i_common i_org i_country +
+  length_of_x509_validity () +
+  length_of_aliasKeyTBS_subject s_common s_org s_country +
+  length_of_subjectPublicKeyInfo +
+  length_of_x509_extensions (length_of_aliasKeyTBS_extensions ku keyID version)
+  <= asn1_value_length_max_of_type SEQUENCE
 
 let length_of_aliasKeyTBS_payload
   (serialNumber: x509_serialNumber_t)
@@ -307,16 +336,44 @@ let length_of_aliasKeyTBS_payload
   (s_org:     x509_RDN_x520_attribute_string_t ORGANIZATION IA5_STRING)
   (s_country: x509_RDN_x520_attribute_string_t COUNTRY      PRINTABLE_STRING)
   (ku: key_usage_payload_t)
-  (version: datatype_of_asn1_type INTEGER)
-: GTot (nat)
-= length_of_x509_version () +
+  (keyID: datatype_of_asn1_type OCTET_STRING)
+  (version: datatype_of_asn1_type INTEGER
+            { valid_aliasKeyTBS_ingredients
+                serialNumber
+                i_common i_org i_country
+                s_common s_org s_country
+                ku keyID version })
+: GTot (asn1_value_length_of_type SEQUENCE)
+= //lemma_aliasKeyTBS_extensions_ingredients_valid ku version;
+  length_of_x509_version () +
   length_of_x509_serialNumber serialNumber +
   length_of_algorithmIdentifier () +
   length_of_aliasKeyTBS_issuer i_common i_org i_country +
   length_of_x509_validity () +
   length_of_aliasKeyTBS_subject s_common s_org s_country +
   length_of_subjectPublicKeyInfo +
-  length_of_x509_extensions (length_of_aliasKeyTBS_extensions ku version)
+  length_of_x509_extensions (length_of_aliasKeyTBS_extensions ku keyID version)
+
+// #push-options "--z3rlimit 1024"
+// let lemma_aliasKeyTBS_ingredients_valid
+//   (serialNumber: x509_serialNumber_t)
+//   (i_common:  x509_RDN_x520_attribute_string_t COMMON_NAME  IA5_STRING)
+//   (i_org:     x509_RDN_x520_attribute_string_t ORGANIZATION IA5_STRING)
+//   (i_country: x509_RDN_x520_attribute_string_t COUNTRY      PRINTABLE_STRING)
+//   (s_common:  x509_RDN_x520_attribute_string_t COMMON_NAME  IA5_STRING)
+//   (s_org:     x509_RDN_x520_attribute_string_t ORGANIZATION IA5_STRING)
+//   (s_country: x509_RDN_x520_attribute_string_t COUNTRY      PRINTABLE_STRING)
+//   (ku: key_usage_payload_t)
+//   (version: datatype_of_asn1_type INTEGER)
+// : Lemma (
+//   valid_aliasKeyTBS_ingredients
+//     serialNumber
+//     i_common i_org i_country
+//     s_common s_org s_country
+//     ku version
+// )
+// = lemma_aliasKeyTBS_extensions_ingredients_valid ku version
+// #pop-options
 
 let len_of_aliasKeyTBS_payload
   (serialNumber: x509_serialNumber_t)
@@ -327,19 +384,19 @@ let len_of_aliasKeyTBS_payload
   (s_org:     x509_RDN_x520_attribute_string_t ORGANIZATION IA5_STRING)
   (s_country: x509_RDN_x520_attribute_string_t COUNTRY      PRINTABLE_STRING)
   (ku: key_usage_payload_t)
+  (keyID: datatype_of_asn1_type OCTET_STRING)
   (version: datatype_of_asn1_type INTEGER
-            { length_of_aliasKeyTBS_payload
+            { valid_aliasKeyTBS_ingredients
                 serialNumber
                 i_common i_org i_country
                 s_common s_org s_country
-                ku version
-              <= asn1_value_length_max_of_type SEQUENCE })
+                ku keyID version })
 : Tot (len: asn1_TLV_int32_of_type SEQUENCE
             { v len == length_of_aliasKeyTBS_payload
                          serialNumber
                          i_common i_org i_country
                          s_common s_org s_country
-                         ku version })
+                         ku keyID version })
 = len_of_x509_version () +
   len_of_x509_serialNumber serialNumber +
   len_of_algorithmIdentifier () +
@@ -347,26 +404,73 @@ let len_of_aliasKeyTBS_payload
   len_of_x509_validity () +
   len_of_aliasKeyTBS_subject s_common s_org s_country +
   len_of_subjectPublicKeyInfo +
-  len_of_x509_extensions (len_of_aliasKeyTBS_extensions ku version)
+  len_of_x509_extensions (len_of_aliasKeyTBS_extensions ku keyID version)
 
 #restart-solver
-#push-options "--z3rlimit 512"
-let lemma_serialize_aliasKeyTBS_payload_size
-  (x: aliasKeyTBS_payload_t)
-: Lemma (
-  let riot_version = RIoT.X509.Extension.(x.aliasKeyTBS_extensions.aliasKeyTBS_extensions_riot.x509_extValue_riot.riot_version) in
-  let ku = (snd x.aliasKeyTBS_extensions.aliasKeyTBS_extensions_key_usage) in
-  (* unfold *)
+#push-options "--z3rlimit 1024"
+let predicate_serialize_aliasKeyTBS_payload_size_unfold
+  (x: aliasKeyTBS_payload_t
+      { valid_aliasKeyTBS_ingredients
+          x.aliasKeyTBS_serialNumber
+          (get_RDN_x520_attribute_string x.aliasKeyTBS_issuer.aliasKeyTBS_issuer_Common)
+          (get_RDN_x520_attribute_string x.aliasKeyTBS_issuer.aliasKeyTBS_issuer_Organization)
+          (get_RDN_x520_attribute_string x.aliasKeyTBS_issuer.aliasKeyTBS_issuer_Country)
+          (get_RDN_x520_attribute_string x.aliasKeyTBS_subject.aliasKeyTBS_subject_Common)
+          (get_RDN_x520_attribute_string x.aliasKeyTBS_subject.aliasKeyTBS_subject_Organization)
+          (get_RDN_x520_attribute_string x.aliasKeyTBS_subject.aliasKeyTBS_subject_Country)
+          (snd x.aliasKeyTBS_extensions.aliasKeyTBS_extensions_key_usage)
+          (snd x.aliasKeyTBS_extensions.aliasKeyTBS_extensions_authKeyID)
+          RIoT.X509.Extension.(x.aliasKeyTBS_extensions.aliasKeyTBS_extensions_riot.x509_extValue_riot.riot_version) })
+: Type0
+=
   length_of_opaque_serialization (serialize_aliasKeyTBS_payload) x ==
   length_of_opaque_serialization (serialize_x509_version)             x.aliasKeyTBS_version      +
   length_of_opaque_serialization (serialize_x509_serialNumber)        x.aliasKeyTBS_serialNumber +
   length_of_opaque_serialization (serialize_algorithmIdentifier)      x.aliasKeyTBS_signatureAlg +
-  length_of_opaque_serialization (serialize_aliasKeyTBS_issuer)       x.aliasKeyTBS_issuer     +
+  length_of_opaque_serialization (serialize_aliasKeyTBS_issuer)       x.aliasKeyTBS_issuer       +
   length_of_opaque_serialization (serialize_x509_validity)            x.aliasKeyTBS_validity     +
-  length_of_opaque_serialization (serialize_aliasKeyTBS_subject)      x.aliasKeyTBS_subject     +
+  length_of_opaque_serialization (serialize_aliasKeyTBS_subject)      x.aliasKeyTBS_subject      +
   length_of_opaque_serialization (serialize_subjectPublicKeyInfo)     x.aliasKeyTBS_aliasKey_pub +
   length_of_opaque_serialization (serialize_x509_extensions_TLV
-                                  serialize_aliasKeyTBS_extensions)   x.aliasKeyTBS_extensions /\
+                                  serialize_aliasKeyTBS_extensions)   x.aliasKeyTBS_extensions
+
+let lemma_serialize_aliasKeyTBS_payload_size
+  (x: aliasKeyTBS_payload_t
+      { valid_aliasKeyTBS_ingredients
+          x.aliasKeyTBS_serialNumber
+          (get_RDN_x520_attribute_string x.aliasKeyTBS_issuer.aliasKeyTBS_issuer_Common)
+          (get_RDN_x520_attribute_string x.aliasKeyTBS_issuer.aliasKeyTBS_issuer_Organization)
+          (get_RDN_x520_attribute_string x.aliasKeyTBS_issuer.aliasKeyTBS_issuer_Country)
+          (get_RDN_x520_attribute_string x.aliasKeyTBS_subject.aliasKeyTBS_subject_Common)
+          (get_RDN_x520_attribute_string x.aliasKeyTBS_subject.aliasKeyTBS_subject_Organization)
+          (get_RDN_x520_attribute_string x.aliasKeyTBS_subject.aliasKeyTBS_subject_Country)
+          (snd x.aliasKeyTBS_extensions.aliasKeyTBS_extensions_key_usage)
+          (snd x.aliasKeyTBS_extensions.aliasKeyTBS_extensions_authKeyID)
+          RIoT.X509.Extension.(x.aliasKeyTBS_extensions.aliasKeyTBS_extensions_riot.x509_extValue_riot.riot_version) })
+: Lemma (
+  // let _ = lemma_aliasKeyTBS_ingredients_valid
+  //           (x.aliasKeyTBS_serialNumber)
+  //           (get_RDN_x520_attribute_string x.aliasKeyTBS_issuer.aliasKeyTBS_issuer_Common)
+  //           (get_RDN_x520_attribute_string x.aliasKeyTBS_issuer.aliasKeyTBS_issuer_Organization)
+  //           (get_RDN_x520_attribute_string x.aliasKeyTBS_issuer.aliasKeyTBS_issuer_Country)
+  //           (get_RDN_x520_attribute_string x.aliasKeyTBS_subject.aliasKeyTBS_subject_Common)
+  //           (get_RDN_x520_attribute_string x.aliasKeyTBS_subject.aliasKeyTBS_subject_Organization)
+  //           (get_RDN_x520_attribute_string x.aliasKeyTBS_subject.aliasKeyTBS_subject_Country)
+  //           ku
+  //           riot_version in
+  // (* unfold *)
+  // let l = serialize_x509_version `length_of_opaque_serialization` x.aliasKeyTBS_version in
+  lemma_serialize_aliasKeyTBS_payload_unfold x;
+    lemma_serialize_x509_version_size_exact x.aliasKeyTBS_version;
+    lemma_serialize_x509_serialNumber_size x.aliasKeyTBS_serialNumber;
+    lemma_serialize_algorithmIdentifier_size_exact x.aliasKeyTBS_signatureAlg;
+    lemma_serialize_aliasKeyTBS_issuer_size_exact x.aliasKeyTBS_issuer;
+    lemma_serialize_x509_validity_size_exact x.aliasKeyTBS_validity;
+    lemma_serialize_aliasKeyTBS_subject_size_exact x.aliasKeyTBS_subject;
+    lemma_serialize_subjectPublicKeyInfo_size_exact x.aliasKeyTBS_aliasKey_pub;
+    lemma_serialize_x509_extensions_TLV_size serialize_aliasKeyTBS_extensions x.aliasKeyTBS_extensions;
+      lemma_serialize_aliasKeyTBS_extensions_size_exact x.aliasKeyTBS_extensions;
+  predicate_serialize_aliasKeyTBS_payload_size_unfold x /\
   (* exact size *)
   length_of_opaque_serialization (serialize_aliasKeyTBS_payload) x
   == length_of_aliasKeyTBS_payload
@@ -377,10 +481,20 @@ let lemma_serialize_aliasKeyTBS_payload_size
        (get_RDN_x520_attribute_string x.aliasKeyTBS_subject.aliasKeyTBS_subject_Common)
        (get_RDN_x520_attribute_string x.aliasKeyTBS_subject.aliasKeyTBS_subject_Organization)
        (get_RDN_x520_attribute_string x.aliasKeyTBS_subject.aliasKeyTBS_subject_Country)
-       ku
-       riot_version
+       (snd x.aliasKeyTBS_extensions.aliasKeyTBS_extensions_key_usage)
+       (snd x.aliasKeyTBS_extensions.aliasKeyTBS_extensions_authKeyID)
+       RIoT.X509.Extension.(x.aliasKeyTBS_extensions.aliasKeyTBS_extensions_riot.x509_extValue_riot.riot_version) /\
+  True
 )
-= lemma_serialize_aliasKeyTBS_payload_unfold x;
+= // Classical.forall_intro_2 (lemma_aliasKeyTBS_ingredients_valid
+  //           (x.aliasKeyTBS_serialNumber)
+  //           (get_RDN_x520_attribute_string x.aliasKeyTBS_issuer.aliasKeyTBS_issuer_Common)
+  //           (get_RDN_x520_attribute_string x.aliasKeyTBS_issuer.aliasKeyTBS_issuer_Organization)
+  //           (get_RDN_x520_attribute_string x.aliasKeyTBS_issuer.aliasKeyTBS_issuer_Country)
+  //           (get_RDN_x520_attribute_string x.aliasKeyTBS_subject.aliasKeyTBS_subject_Common)
+  //           (get_RDN_x520_attribute_string x.aliasKeyTBS_subject.aliasKeyTBS_subject_Organization)
+  //           (get_RDN_x520_attribute_string x.aliasKeyTBS_subject.aliasKeyTBS_subject_Country));
+  lemma_serialize_aliasKeyTBS_payload_unfold x;
     lemma_serialize_x509_version_size_exact x.aliasKeyTBS_version;
     lemma_serialize_x509_serialNumber_size x.aliasKeyTBS_serialNumber;
     lemma_serialize_algorithmIdentifier_size_exact x.aliasKeyTBS_signatureAlg;
@@ -428,13 +542,13 @@ let length_of_aliasKeyTBS
   (s_org:     x509_RDN_x520_attribute_string_t ORGANIZATION IA5_STRING)
   (s_country: x509_RDN_x520_attribute_string_t COUNTRY      PRINTABLE_STRING)
   (ku: key_usage_payload_t)
+  (keyID: datatype_of_asn1_type OCTET_STRING)
   (version: datatype_of_asn1_type INTEGER
-            { length_of_aliasKeyTBS_payload
+            { valid_aliasKeyTBS_ingredients
                 serialNumber
                 i_common i_org i_country
                 s_common s_org s_country
-                ku version
-              <= asn1_value_length_max_of_type SEQUENCE })
+                ku keyID version })
 : GTot (asn1_TLV_length_of_type SEQUENCE)
 = length_of_TLV
     (SEQUENCE)
@@ -442,7 +556,7 @@ let length_of_aliasKeyTBS
       serialNumber
       i_common i_org i_country
       s_common s_org s_country
-      ku version)
+      ku keyID version)
 
 #restart-solver
 let len_of_aliasKeyTBS
@@ -454,35 +568,48 @@ let len_of_aliasKeyTBS
   (s_org:     x509_RDN_x520_attribute_string_t ORGANIZATION IA5_STRING)
   (s_country: x509_RDN_x520_attribute_string_t COUNTRY      PRINTABLE_STRING)
   (ku: key_usage_payload_t)
+  (keyID: datatype_of_asn1_type OCTET_STRING)
   (version: datatype_of_asn1_type INTEGER
-            { length_of_aliasKeyTBS_payload
+            { valid_aliasKeyTBS_ingredients
                 serialNumber
                 i_common i_org i_country
                 s_common s_org s_country
-                ku version
-              <= asn1_value_length_max_of_type SEQUENCE })
-// : Tot (len: asn1_TLV_length_of_type SEQUENCE
-//              { v len == length_of_aliasKeyTBS
-//                           serialNumber
-//                           i_common i_org i_country
-//                           s_common s_org s_country
-//                           ku version })
+                ku keyID version })
+: Tot (len: asn1_TLV_int32_of_type SEQUENCE
+             { v len == length_of_aliasKeyTBS
+                          serialNumber
+                          i_common i_org i_country
+                          s_common s_org s_country
+                          ku keyID version })
 = len_of_TLV
     (SEQUENCE)
     (len_of_aliasKeyTBS_payload
       serialNumber
       i_common i_org i_country
       s_common s_org s_country
-      ku version)
+      ku keyID version)
+
+let valid_aliasKeyTBS
+  (x: aliasKeyTBS_t)
+: Type0
+= valid_aliasKeyTBS_ingredients
+          x.aliasKeyTBS_serialNumber
+          (get_RDN_x520_attribute_string x.aliasKeyTBS_issuer.aliasKeyTBS_issuer_Common)
+          (get_RDN_x520_attribute_string x.aliasKeyTBS_issuer.aliasKeyTBS_issuer_Organization)
+          (get_RDN_x520_attribute_string x.aliasKeyTBS_issuer.aliasKeyTBS_issuer_Country)
+          (get_RDN_x520_attribute_string x.aliasKeyTBS_subject.aliasKeyTBS_subject_Common)
+          (get_RDN_x520_attribute_string x.aliasKeyTBS_subject.aliasKeyTBS_subject_Organization)
+          (get_RDN_x520_attribute_string x.aliasKeyTBS_subject.aliasKeyTBS_subject_Country)
+          (snd x.aliasKeyTBS_extensions.aliasKeyTBS_extensions_key_usage)
+          (snd x.aliasKeyTBS_extensions.aliasKeyTBS_extensions_authKeyID)
+          RIoT.X509.Extension.(x.aliasKeyTBS_extensions.aliasKeyTBS_extensions_riot.x509_extValue_riot.riot_version)
 
 #restart-solver
-#push-options "--z3rlimit 512"
 let lemma_serialize_aliasKeyTBS_size_exact
-  (x: aliasKeyTBS_t)
+  (x: aliasKeyTBS_t
+      { valid_aliasKeyTBS x })
 : Lemma (
-  let riot_version = RIoT.X509.Extension.(x.aliasKeyTBS_extensions.aliasKeyTBS_extensions_riot.x509_extValue_riot.riot_version) in
-  let ku = (snd x.aliasKeyTBS_extensions.aliasKeyTBS_extensions_key_usage) in
-  let _ = lemma_serialize_aliasKeyTBS_payload_size x in
+  lemma_serialize_aliasKeyTBS_payload_size x;
   (* exact size *)
   length_of_opaque_serialization (serialize_aliasKeyTBS) x
   == length_of_aliasKeyTBS
@@ -493,12 +620,12 @@ let lemma_serialize_aliasKeyTBS_size_exact
        (get_RDN_x520_attribute_string x.aliasKeyTBS_subject.aliasKeyTBS_subject_Common)
        (get_RDN_x520_attribute_string x.aliasKeyTBS_subject.aliasKeyTBS_subject_Organization)
        (get_RDN_x520_attribute_string x.aliasKeyTBS_subject.aliasKeyTBS_subject_Country)
-       ku
-       riot_version
+       (snd x.aliasKeyTBS_extensions.aliasKeyTBS_extensions_key_usage)
+       (snd x.aliasKeyTBS_extensions.aliasKeyTBS_extensions_authKeyID)
+       RIoT.X509.Extension.(x.aliasKeyTBS_extensions.aliasKeyTBS_extensions_riot.x509_extValue_riot.riot_version)
 )
 = lemma_serialize_aliasKeyTBS_size x;
     lemma_serialize_aliasKeyTBS_payload_size x
-#pop-options
 
 (* low *)
 let serialize32_aliasKeyTBS_payload_backwards
@@ -523,6 +650,8 @@ let serialize32_aliasKeyTBS_payload_backwards
   (* g1 *) (synth_aliasKeyTBS_payload_t')
   (* g1'*) (synth_aliasKeyTBS_payload_t')
   (* prf*) ()
+  `coerce_serializer32_backwards serialize_aliasKeyTBS_payload`
+  ()
 
 let serialize32_aliasKeyTBS_backwards
 : serializer32_backwards (serialize_aliasKeyTBS)
@@ -532,7 +661,6 @@ let serialize32_aliasKeyTBS_backwards
              (serialize32_aliasKeyTBS_payload_backwards))
   (* prf*) ()
 
-
 (* helpers *)
 #restart-solver
 let x509_get_AliasKeyTBS
@@ -540,26 +668,24 @@ let x509_get_AliasKeyTBS
   (serialNumber: x509_serialNumber_t)
   (i_common:  x509_RDN_x520_attribute_string_t COMMON_NAME  IA5_STRING)
   (i_org:     x509_RDN_x520_attribute_string_t ORGANIZATION IA5_STRING)
-  (i_country: x509_RDN_x520_attribute_string_t COUNTRY      PRINTABLE_STRING
-              { length_of_aliasKeyTBS_issuer_payload i_common i_org i_country
-                <= asn1_value_length_max_of_type SEQUENCE })
+  (i_country: x509_RDN_x520_attribute_string_t COUNTRY      PRINTABLE_STRING)
   (notBefore: datatype_of_asn1_type Generalized_Time)
   (notAfter : datatype_of_asn1_type Generalized_Time)
   (s_common:  x509_RDN_x520_attribute_string_t COMMON_NAME  IA5_STRING)
   (s_org:     x509_RDN_x520_attribute_string_t ORGANIZATION IA5_STRING)
   (s_country: x509_RDN_x520_attribute_string_t COUNTRY      PRINTABLE_STRING)
   (ku: key_usage_payload_t)
+  (keyID: datatype_of_asn1_type OCTET_STRING)
   (version: datatype_of_asn1_type INTEGER
-            { length_of_aliasKeyTBS_payload
+            { valid_aliasKeyTBS_ingredients
                 serialNumber
                 i_common i_org i_country
                 s_common s_org s_country
-                ku version
-              <= asn1_value_length_max_of_type SEQUENCE })
+                ku keyID version })
   (fwid: B32.lbytes32 32ul)
   (deviceIDPub: B32.lbytes32 32ul)
   (aliasKeyPub: B32.lbytes32 32ul)
-: Tot (aliasKeyTBS_t)
+: Tot (x: aliasKeyTBS_t { valid_aliasKeyTBS x })
 =
   let signatureAlg: algorithmIdentifier_t = x509_get_algorithmIdentifier () in
   (* Prf *) lemma_serialize_algorithmIdentifier_size_exact signatureAlg;
@@ -593,6 +719,7 @@ let x509_get_AliasKeyTBS
 
   let extensions = x509_get_aliasKeyTBS_extensions
                                  ku
+                                 keyID
                                  version
                                  fwid
                                  deviceIDPub in
