src/riot/asn1/ASN1.Spec.Value.BOOLEAN.fst
@@ -283,3 +283,49 @@ let lemma_serialize_asn1_boolean_TLV_size
   Seq.length (serialize serialize_asn1_boolean_TLV value) == 3)
 = parser_kind_prop_equiv parse_asn1_boolean_TLV_kind parse_asn1_boolean_TLV;
   lemma_serialize_asn1_boolean_TLV_unfold value
+
+let filter_asn1_boolean_true
+  (x: datatype_of_asn1_type BOOLEAN)
+: GTot (bool)
+= x = true
+
+let asn1_boolean_true_t
+: Type
+= parse_filter_refine filter_asn1_boolean_true
+
+let asn1_boolean_true: asn1_boolean_true_t = true
+
+let parse_asn1_boolean_TLV_true
+: parser parse_asn1_boolean_TLV_kind asn1_boolean_true_t
+= parse_asn1_boolean_TLV
+  `parse_filter`
+  filter_asn1_boolean_true
+
+let serialize_asn1_boolean_TLV_true
+: serializer parse_asn1_boolean_TLV_true
+= serialize_asn1_boolean_TLV
+  `serialize_filter`
+  filter_asn1_boolean_true
+
+let filter_asn1_boolean_false
+  (x: datatype_of_asn1_type BOOLEAN)
+: GTot (bool)
+= x = false
+
+let asn1_boolean_false_t
+: Type
+= parse_filter_refine filter_asn1_boolean_false
+
+let asn1_boolean_false: asn1_boolean_false_t = false
+
+let parse_asn1_boolean_TLV_false
+: parser parse_asn1_boolean_TLV_kind asn1_boolean_false_t
+= parse_asn1_boolean_TLV
+  `parse_filter`
+  filter_asn1_boolean_false
+
+let serialize_asn1_boolean_TLV_false
+: serializer parse_asn1_boolean_TLV_false
+= serialize_asn1_boolean_TLV
+  `serialize_filter`
+  filter_asn1_boolean_false
