src/riot/x509/X509.ExtFields.BasicConstraints.fst
@@ -5,141 +5,519 @@ open LowParse.Spec.Combinators
 
 open ASN1.Base
 open ASN1.Spec
+open ASN1.Low
 
 open X509.Base
+open X509.BasicFields.Extension2
 
 module B32 = FStar.Bytes
 
 open FStar.Integers
 
-(* Not using for now
+#set-options "--z3rlimit 64 --fuel 0 --ifuel 0"
 
-let x509_basic_constraints_t
-  (hasLenField: bool)
-= if hasLenField then
-  ( tuple2 (datatype_of_asn1_type BOOLEAN) (datatype_of_asn1_type INTEGER) )
+(* RFC 5280  4.2.1.9.  Basic Constraints
+   The basic constraints extension identifies whether the subject of the
+   certificate is a CA and the maximum depth of valid certification
+   paths that include this certificate.
+
+   The cA boolean indicates whether the certified public key may be used
+   to verify certificate signatures.  If the cA boolean is not asserted,
+   then the keyCertSign bit in the key usage extension MUST NOT be
+   asserted.  If the basic constraints extension is not present in a
+   version 3 certificate, or the extension is present but the cA boolean
+   is not asserted, then the certified public key MUST NOT be used to
+   verify certificate signatures.
+
+   The pathLenConstraint field is meaningful only if the cA boolean is
+   asserted and the key usage extension, if present, asserts the
+   keyCertSign bit (Section 4.2.1.3).  In this case, it gives the
+   maximum number of non-self-issued intermediate certificates that may
+   follow this certificate in a valid certification path.  (Note: The
+   last certificate in the certification path is not an intermediate
+   certificate, and is not included in this limit.  Usually, the last
+   certificate is an end entity certificate, but it can be a CA
+   certificate.)  A pathLenConstraint of zero indicates that no non-
+   self-issued intermediate CA certificates may follow in a valid
+   certification path.  Where it appears, the pathLenConstraint field
+   MUST be greater than or equal to zero.  Where pathLenConstraint does
+   not appear, no limit is imposed.
+
+   Conforming CAs MUST include this extension in all CA certificates
+   that contain public keys used to validate digital signatures on
+   certificates and MUST mark the extension as critical in such
+   certificates.  This extension MAY appear as a critical or non-
+   critical extension in CA certificates that contain public keys used
+   exclusively for purposes other than validating digital signatures on
+   certificates.  Such CA certificates include ones that contain public
+   keys used exclusively for validating digital signatures on CRLs and
+   ones that contain key management public keys used with certificate
+   enrollment protocols.  This extension MAY appear as a critical or
+   non-critical extension in end entity certificates.
+
+   CAs MUST NOT include the pathLenConstraint field unless the cA
+   boolean is asserted and the key usage extension asserts the
+   keyCertSign bit.
+
+   id-ce-basicConstraints OBJECT IDENTIFIER ::=  { id-ce 19 }
+
+   BasicConstraints ::= SEQUENCE {
+        cA                      BOOLEAN DEFAULT FALSE,
+        pathLenConstraint       INTEGER (0..MAX) OPTIONAL }
+ *)
+
+noextract inline_for_extraction
+let x509_basicConstraints_extValue_payload_t
+  (isCA: bool)
+= if isCA then
+  ( asn1_boolean_true_t `tuple2` (datatype_of_asn1_type INTEGER) )
   else
-  ( bool )
+  ( asn1_boolean_false_t )
 
-let parse_x509_basic_constraints_kind
-  (hasLenField: bool)
+let parse_x509_basicConstraints_extValue_payload_kind
+  (isCA: bool)
 : k: parser_kind {Mkparser_kind'?.parser_kind_subkind k == Some ParserStrong}
-= if hasLenField then
+= if isCA then
   ( parse_asn1_TLV_kind_of_type BOOLEAN
     `and_then_kind`
     parse_asn1_TLV_kind_of_type INTEGER )
   else
   ( parse_asn1_TLV_kind_of_type BOOLEAN )
 
-let parse_x509_basic_constraints
-  (hasLenField: bool)
-: parser (parse_x509_basic_constraints_kind hasLenField) (x509_basic_constraints_t hasLenField)
-= if hasLenField then
-  ( parse_asn1_TLV_of_type BOOLEAN
+let parse_x509_basicConstraints_extValue_payload
+  (isCA: bool)
+: parser (parse_x509_basicConstraints_extValue_payload_kind isCA) (x509_basicConstraints_extValue_payload_t isCA)
+= if isCA then
+  ( parse_asn1_boolean_TLV_true
     `nondep_then`
     parse_asn1_TLV_of_type INTEGER )
   else
-  ( parse_asn1_TLV_of_type BOOLEAN )
+  ( parse_asn1_boolean_TLV_false )
 
-let serialize_x509_basic_constraints
-  (hasLenField: bool)
-: serializer (parse_x509_basic_constraints hasLenField)
-= if hasLenField then
-  ( serialize_asn1_TLV_of_type BOOLEAN
+let serialize_x509_basicConstraints_extValue_payload
+  (isCA: bool)
+: serializer (parse_x509_basicConstraints_extValue_payload isCA)
+= if isCA then
+  ( serialize_asn1_boolean_TLV_true
     `serialize_nondep_then`
     serialize_asn1_TLV_of_type INTEGER )
   else
-  ( serialize_asn1_TLV_of_type BOOLEAN )
+  ( serialize_asn1_boolean_TLV_false )
 
-let lemma_serialize_x509_basic_constraints_unfold
-  (hasLenField: bool)
-  (x: x509_basic_constraints_t hasLenField)
+noextract inline_for_extraction
+let serialize32_x509_basicConstraints_extValue_payload_backwards
+  (isCA: bool)
+: serializer32_backwards (serialize_x509_basicConstraints_extValue_payload isCA)
+= if isCA then
+  ( serialize32_asn1_boolean_TLV_true_backwards ()
+    `serialize32_nondep_then_backwards`
+    serialize32_asn1_TLV_backwards_of_type INTEGER )
+  else
+  ( serialize32_asn1_boolean_TLV_false_backwards () )
+
+let lemma_serialize_x509_basicConstraints_extValue_payload_unfold
+  (isCA: bool)
+  (x: x509_basicConstraints_extValue_payload_t isCA)
 : Lemma (
-  serialize (serialize_x509_basic_constraints hasLenField) x ==
-  ( if hasLenField then
-    ( let x = x <: datatype_of_asn1_type BOOLEAN `tuple2` datatype_of_asn1_type INTEGER in
-      serialize (serialize_asn1_TLV_of_type BOOLEAN) (fst x)
+  serialize (serialize_x509_basicConstraints_extValue_payload isCA) x ==
+  ( if isCA then
+    ( let x = x <: asn1_boolean_true_t `tuple2` datatype_of_asn1_type INTEGER in
+      serialize (serialize_asn1_boolean_TLV_true) (fst x)
       `Seq.append`
       serialize (serialize_asn1_TLV_of_type INTEGER) (snd x) )
     else
-    ( let x = x <: datatype_of_asn1_type BOOLEAN in
-      serialize (serialize_asn1_TLV_of_type BOOLEAN) x ) )
+    ( let x = x <: asn1_boolean_false_t in
+      serialize (serialize_asn1_boolean_TLV_false) x ) )
 )
-= if hasLenField then
+= if isCA then
   ( serialize_nondep_then_eq
-    (* s1 *) (serialize_asn1_TLV_of_type BOOLEAN)
+    (* s1 *) (serialize_asn1_boolean_TLV_true)
     (* s2 *) (serialize_asn1_TLV_of_type INTEGER)
     (* in *) x )
   else
   ( () )
 
-let lemma_serialize_x509_basic_constraints_size
-  (hasLenField: bool)
-  (x: x509_basic_constraints_t hasLenField)
-: Lemma (
-  Seq.length (serialize (serialize_x509_basic_constraints hasLenField) x) ==
-  ( if hasLenField then
-    ( let x = x <: datatype_of_asn1_type BOOLEAN `tuple2` datatype_of_asn1_type INTEGER in
-      length_of_asn1_primitive_TLV (fst x) +
-      length_of_asn1_primitive_TLV (snd x) )
-    else
-    ( let x = x <: datatype_of_asn1_type BOOLEAN in
-      length_of_asn1_primitive_TLV x ) )
-)
-= lemma_serialize_x509_basic_constraints_unfold hasLenField x
+let length_of_x509_basicConstraints_extValue_payload_hasLen
+  (pathLen: datatype_of_asn1_type INTEGER)
+: GTot (nat)
+= length_of_asn1_primitive_TLV true +
+  length_of_asn1_primitive_TLV pathLen
 
-let parse_x509_basic_constraints_sequence_TLV
-  (hasLenField: bool)
-= parse_asn1_sequence_TLV
-    (OID_BASIC_CONSTRAINTS
-     `serialize_envelop_OID_with`
-     serialize_x509_basic_constraints hasLenField)
-
-let serialize_x509_basic_constraints_sequence_TLV
-  (hasLenField: bool)
-: serializer (parse_x509_basic_constraints_sequence_TLV hasLenField)
-= serialize_asn1_sequence_TLV
-    (OID_BASIC_CONSTRAINTS
-     `serialize_envelop_OID_with`
-     serialize_x509_basic_constraints hasLenField)
-
-let lemma_serialize_x509_basic_constraints_sequence_TLV_unfold
-  (hasLenField: bool)
-= lemma_serialize_asn1_sequence_TLV_unfold
-    (OID_BASIC_CONSTRAINTS
-     `serialize_envelop_OID_with`
-     serialize_x509_basic_constraints hasLenField)
-
-let lemma_serialize_x509_basic_constraints_sequence_TLV_size
-  (hasLenField: bool)
-= lemma_serialize_asn1_sequence_TLV_size
-    (OID_BASIC_CONSTRAINTS
-     `serialize_envelop_OID_with`
-     serialize_x509_basic_constraints hasLenField)
-
-open ASN1.Low
-
-let x509_basic_constraints_t_inbound
-  (hasLenField: bool)
-= inbound_sequence_value_of (serialize_x509_basic_constraints hasLenField)
-
-noextract
-let serialize32_x509_basic_constraints_backwards
-  (hasLenField: bool)
-: serializer32_backwards (serialize_x509_basic_constraints hasLenField)
-= if hasLenField then
-  ( serialize32_asn1_TLV_backwards_of_type BOOLEAN
-    `serialize32_nondep_then_backwards`
-    serialize32_asn1_TLV_backwards_of_type INTEGER )
+let length_of_x509_basicConstraints_extValue_payload
+  (isCA: bool)
+: GTot ( if isCA then
+         ( datatype_of_asn1_type INTEGER -> GTot (asn1_value_length_of_type SEQUENCE) )
+         else
+         ( asn1_value_length_of_type SEQUENCE ) )
+= if isCA then
+  ( length_of_x509_basicConstraints_extValue_payload_hasLen )
   else
-  ( serialize32_asn1_TLV_backwards_of_type BOOLEAN )
+  ( length_of_asn1_primitive_TLV false )
 
-let serialize32_x509_basic_constraints_sequence_TLV_backwards
-  (hasLenField: bool)
-: serializer32_backwards (serialize_x509_basic_constraints_sequence_TLV hasLenField)
-= serialize32_asn1_sequence_TLV_backwards
-  (* s32 *) (OID_BASIC_CONSTRAINTS
-             `serialize32_envelop_OID_with_backwards`
-             serialize32_x509_basic_constraints_backwards hasLenField)
+// let valid_x509_basicConstraints_extValue_payload
+//   (isCA: bool)
+// : ( if isCA then
+//     ( datatype_of_asn1_type INTEGER -> Type0 )
+//     else
+//     ( Type0 ) )
+// = if isCA then
+//   ( fun (pathLen: datatype_of_asn1_type INTEGER) ->
+//     length_of_x509_basicConstraints_extValue_payload true pathLen
+//     <= asn1_value_length_max_of_type OCTET_STRING )
+//   <: datatype_of_asn1_type INTEGER -> Type0
+//   else
+//   ( True )
 
-let _ = assert (length_of_oid OID_EC_GRP_SECP256R1 == 6)
+let len_of_x509_basicConstraints_extValue_payload_hasLen
+  (pathLen: datatype_of_asn1_type INTEGER)
+            // { valid_x509_basicConstraints_extValue_payload true pathLen })
+: Tot (len: asn1_value_int32_of_type SEQUENCE
+            { v len == length_of_x509_basicConstraints_extValue_payload_hasLen pathLen })
+= len_of_asn1_primitive_TLV true +
+  len_of_asn1_primitive_TLV pathLen
+
+noextract inline_for_extraction
+let len_of_x509_basicConstraints_extValue_payload
+  (isCA: bool)
+: Tot ( if isCA then
+         ( (pathLen: datatype_of_asn1_type INTEGER)
+           -> Tot (len: asn1_value_int32_of_type SEQUENCE
+                        { v len == length_of_x509_basicConstraints_extValue_payload true pathLen }) )
+         else
+         ( len: asn1_value_int32_of_type SEQUENCE
+                { v len == length_of_x509_basicConstraints_extValue_payload false } ) )
+= if isCA then
+  ( len_of_x509_basicConstraints_extValue_payload_hasLen )
+  else
+  ( len_of_asn1_primitive_TLV false )
+
+let lemma_serialize_x509_basicConstraints_extValue_payload_size
+  (isCA: bool)
+  (x: x509_basicConstraints_extValue_payload_t isCA)
+: Lemma (
+  Seq.length (serialize (serialize_x509_basicConstraints_extValue_payload isCA) x) ==
+  ( if isCA then
+    ( let x = x <: asn1_boolean_true_t `tuple2` datatype_of_asn1_type INTEGER in
+      length_of_x509_basicConstraints_extValue_payload true (snd x)  )
+    else
+    ( length_of_x509_basicConstraints_extValue_payload false ) )
+)
+= lemma_serialize_x509_basicConstraints_extValue_payload_unfold isCA x
+
+(* extValue *)
+
+noextract inline_for_extraction
+let x509_basicConstraints_extValue_t
+  (isCA: bool)
+: Type
+= inbound_sequence_value_of
+  (**) (serialize_x509_basicConstraints_extValue_payload isCA)
+
+let parse_x509_basicConstraints_extValue
+  (isCA: bool)
+: parser _ (x509_basicConstraints_extValue_t isCA)
+= x509_basicConstraints_extValue_t isCA
+  `coerce_parser`
+  parse_asn1_sequence_TLV
+  (**) (serialize_x509_basicConstraints_extValue_payload isCA)
+
+let serialize_x509_basicConstraints_extValue
+  (isCA: bool)
+: serializer (parse_x509_basicConstraints_extValue isCA)
+= coerce_parser_serializer
+    (parse_x509_basicConstraints_extValue isCA)
+    (serialize_asn1_sequence_TLV
+    (**) (serialize_x509_basicConstraints_extValue_payload isCA))
+    ()
+
+noextract inline_for_extraction
+let serialize32_x509_basicConstraints_extValue_backwards
+  (isCA: bool)
+: serializer32_backwards (serialize_x509_basicConstraints_extValue isCA)
+= coerce_serializer32_backwards
+    (serialize_x509_basicConstraints_extValue isCA)
+    (serialize32_asn1_sequence_TLV_backwards
+    (**) (serialize32_x509_basicConstraints_extValue_payload_backwards isCA))
+    ()
+
+let lemma_serialize_x509_basicConstraints_extValue_unfold
+  (isCA: bool)
+  (x: x509_basicConstraints_extValue_t isCA)
+: Lemma (
+  predicate_serialize_asn1_sequence_TLV_unfold
+    (serialize_x509_basicConstraints_extValue_payload isCA)
+    (x)
+)
+= lemma_serialize_asn1_sequence_TLV_unfold
+    (serialize_x509_basicConstraints_extValue_payload isCA)
+    (x)
+
+let lemma_serialize_x509_basicConstraints_extValue_size
+  (isCA: bool)
+  (x: x509_basicConstraints_extValue_t isCA)
+: Lemma (
+  predicate_serialize_asn1_sequence_TLV_size
+    (serialize_x509_basicConstraints_extValue_payload isCA)
+    (x)
+)
+= lemma_serialize_asn1_sequence_TLV_size
+    (serialize_x509_basicConstraints_extValue_payload isCA)
+    (x)
+
+let length_of_x509_basicConstraints_extValue
+  (isCA: bool)
+: GTot ( if isCA then
+         ( datatype_of_asn1_type INTEGER -> GTot (asn1_value_length_of_type OCTET_STRING) )
+         else
+         ( asn1_value_length_of_type OCTET_STRING ) )
+= if isCA then
+  ( fun (pathLen: datatype_of_asn1_type INTEGER) ->
+      length_of_TLV
+        (SEQUENCE)
+        (length_of_x509_basicConstraints_extValue_payload true pathLen) )
+  else
+  ( length_of_TLV
+      (SEQUENCE)
+      (length_of_x509_basicConstraints_extValue_payload isCA) )
+
+noextract inline_for_extraction
+let len_of_x509_basicConstraints_extValue
+  (isCA: bool)
+: Tot ( if isCA then
+         ( (pathLen: datatype_of_asn1_type INTEGER)
+           -> Tot (len: asn1_value_int32_of_type OCTET_STRING
+                        { v len == length_of_x509_basicConstraints_extValue true pathLen }) )
+        else
+        ( len: asn1_value_int32_of_type OCTET_STRING
+               { v len == length_of_x509_basicConstraints_extValue isCA } ) )
+= if isCA then
+  ( fun (pathLen: datatype_of_asn1_type INTEGER) ->
+      len_of_TLV
+        (SEQUENCE)
+        (len_of_x509_basicConstraints_extValue_payload true pathLen) )
+  else
+  ( len_of_TLV
+      (SEQUENCE)
+      (len_of_x509_basicConstraints_extValue_payload isCA) )
+
+let lemma_serialize_x509_basicConstraints_extValue_size_exact
+  (isCA: bool)
+  (x: x509_basicConstraints_extValue_t isCA)
+: Lemma (
+  lemma_serialize_x509_basicConstraints_extValue_unfold isCA x;
+  lemma_serialize_x509_basicConstraints_extValue_size isCA x;
+    lemma_serialize_x509_basicConstraints_extValue_payload_size isCA x;
+  if isCA then
+  ( let x = x <: asn1_boolean_true_t `tuple2` datatype_of_asn1_type INTEGER in
+    length_of_opaque_serialization (serialize_x509_basicConstraints_extValue isCA) x
+    == length_of_x509_basicConstraints_extValue true (snd x) )
+  else
+  ( length_of_opaque_serialization (serialize_x509_basicConstraints_extValue isCA) x
+    == length_of_x509_basicConstraints_extValue false )
+)
+= lemma_serialize_x509_basicConstraints_extValue_unfold isCA x;
+  lemma_serialize_x509_basicConstraints_extValue_size isCA x;
+    lemma_serialize_x509_basicConstraints_extValue_payload_size isCA x
+
+(* ext *)
+
+noextract inline_for_extraction
+let x509_basicConstraints_t
+  (isCA: bool)
+: Type
+= x509_extension_t
+  (**) (OID_BASIC_CONSTRAINTS)
+  (**) (serialize_x509_basicConstraints_extValue isCA)
+
+let parse_x509_basicConstraints
+  (isCA: bool)
+: parser parse_x509_extension_kind (x509_basicConstraints_t isCA)
+= x509_basicConstraints_t isCA
+  `coerce_parser`
+  parse_x509_extension
+  (**) (OID_BASIC_CONSTRAINTS)
+  (**) (serialize_x509_basicConstraints_extValue isCA)
+
+let serialize_x509_basicConstraints
+  (isCA: bool)
+: serializer (parse_x509_basicConstraints isCA)
+= coerce_parser_serializer
+    (parse_x509_basicConstraints isCA)
+    (serialize_x509_extension
+    (**) (OID_BASIC_CONSTRAINTS)
+    (**) (serialize_x509_basicConstraints_extValue isCA))
+    ()
+
+noextract inline_for_extraction
+let serialize32_x509_basicConstraints_backwards
+  (isCA: bool)
+: serializer32_backwards (serialize_x509_basicConstraints isCA)
+= coerce_serializer32_backwards
+    (_)
+    (serialize32_x509_extension_backwards
+    (**) (OID_BASIC_CONSTRAINTS)
+    (**) (serialize32_x509_basicConstraints_extValue_backwards isCA))
+    ()
+
+let lemma_serialize_x509_basicConstraints_unfold
+  (isCA: bool)
+  (x: x509_basicConstraints_t isCA)
+: Lemma ( predicate_serialize_x509_extension_unfold
+          (**) (OID_BASIC_CONSTRAINTS)
+          (**) (serialize_x509_basicConstraints_extValue isCA)
+          (**) (x) )
+= lemma_serialize_x509_extension_unfold
+  (**) (OID_BASIC_CONSTRAINTS)
+  (**) (serialize_x509_basicConstraints_extValue isCA)
+  (**) (x)
+
+let lemma_serialize_x509_basicConstraints_size
+  (isCA: bool)
+  (x: x509_basicConstraints_t isCA)
+: Lemma ( predicate_serialize_x509_extension_size
+          (**) (OID_BASIC_CONSTRAINTS)
+          (**) (serialize_x509_basicConstraints_extValue isCA)
+          (**) (x) )
+= lemma_serialize_x509_extension_size
+  (**) (OID_BASIC_CONSTRAINTS)
+  (**) (serialize_x509_basicConstraints_extValue isCA)
+  (**) (x)
+
+let length_of_x509_basicConstraints
+  (isCA: bool)
+: GTot ( if isCA then
+         ( datatype_of_asn1_type INTEGER -> GTot (asn1_TLV_length_of_type SEQUENCE) )
+         else
+         ( asn1_TLV_length_of_type SEQUENCE ) )
+= if isCA then
+  ( fun (pathLen: datatype_of_asn1_type INTEGER) ->
+      let x: x509_basicConstraints_extValue_payload_t isCA = (asn1_boolean_true, pathLen) in
+      lemma_serialize_x509_basicConstraints_extValue_size_exact isCA x;
+      lemma_serialize_x509_basicConstraints_extValue_payload_size isCA x;
+      length_of_x509_extension
+        (OID_BASIC_CONSTRAINTS)
+        (serialize_x509_basicConstraints_extValue isCA)
+        (x <: x509_basicConstraints_extValue_t isCA)
+        (length_of_x509_basicConstraints_extValue true pathLen) )
+  else
+  ( let x: x509_basicConstraints_extValue_payload_t isCA = (asn1_boolean_false) in
+    lemma_serialize_x509_basicConstraints_extValue_size_exact isCA x;
+    lemma_serialize_x509_basicConstraints_extValue_payload_size isCA x;
+    length_of_x509_extension
+      (OID_BASIC_CONSTRAINTS)
+      (serialize_x509_basicConstraints_extValue isCA)
+      (x <: x509_basicConstraints_extValue_t isCA)
+      (length_of_x509_basicConstraints_extValue false) )
+
+noextract inline_for_extraction
+let len_of_x509_basicConstraints
+  (isCA: bool)
+: Tot ( if isCA then
+         ( (pathLen: datatype_of_asn1_type INTEGER)
+           -> Tot (len: asn1_TLV_int32_of_type SEQUENCE
+                        { v len == length_of_x509_basicConstraints true pathLen }) )
+        else
+        ( len: asn1_TLV_int32_of_type SEQUENCE
+               { v len == length_of_x509_basicConstraints isCA } ) )
+= if isCA then
+  ( fun (pathLen: datatype_of_asn1_type INTEGER) ->
+      let x: x509_basicConstraints_extValue_payload_t isCA = (asn1_boolean_true, pathLen) in
+      lemma_serialize_x509_basicConstraints_extValue_size_exact isCA x;
+      lemma_serialize_x509_basicConstraints_extValue_payload_size isCA x;
+      len_of_x509_extension
+        (OID_BASIC_CONSTRAINTS)
+        (serialize_x509_basicConstraints_extValue isCA)
+        ((asn1_boolean_true, pathLen) <: x509_basicConstraints_extValue_payload_t isCA)
+        (len_of_x509_basicConstraints_extValue true pathLen) )
+  else
+  ( let x: x509_basicConstraints_extValue_payload_t isCA = (asn1_boolean_false) in
+    lemma_serialize_x509_basicConstraints_extValue_size_exact isCA x;
+    lemma_serialize_x509_basicConstraints_extValue_payload_size isCA x;
+    len_of_x509_extension
+      (OID_BASIC_CONSTRAINTS)
+      (serialize_x509_basicConstraints_extValue isCA)
+      (x <: x509_basicConstraints_extValue_t isCA)
+      (len_of_x509_basicConstraints_extValue false) )
+
+let lemma_serialize_x509_basicConstraints_size_exact
+  (isCA: bool)
+  (ext: x509_basicConstraints_t isCA)
+: Lemma (
+  length_of_opaque_serialization (serialize_x509_basicConstraints isCA) ext ==
+  ( if isCA then
+    ( let x = snd ext <: asn1_boolean_true_t `tuple2` datatype_of_asn1_type INTEGER in
+      length_of_x509_basicConstraints true (snd x) )
+    else
+    ( length_of_x509_basicConstraints false ) )
+)
+= if isCA then
+  ( lemma_serialize_x509_basicConstraints_extValue_size_exact isCA (snd ext);
+    lemma_serialize_x509_basicConstraints_extValue_payload_size isCA (snd ext);
+    lemma_serialize_x509_extension_size_exact
+      (OID_BASIC_CONSTRAINTS)
+      (serialize_x509_basicConstraints_extValue isCA)
+      (ext)
+      (length_of_x509_basicConstraints_extValue true (snd (snd ext <: x509_basicConstraints_extValue_payload_t true))) )
+  else
+  ( lemma_serialize_x509_basicConstraints_extValue_size_exact isCA (snd ext);
+    lemma_serialize_x509_basicConstraints_extValue_payload_size isCA (snd ext);
+    lemma_serialize_x509_extension_size_exact
+      (OID_BASIC_CONSTRAINTS)
+      (serialize_x509_basicConstraints_extValue isCA)
+      (ext)
+      (length_of_x509_basicConstraints_extValue false) )
+
+let x509_get_basicConstraints_isCA
+  (isCA: bool { isCA == true })
+  (criticality: datatype_of_asn1_type BOOLEAN)
+  (pathLen: datatype_of_asn1_type INTEGER)
+: Tot (x509_basicConstraints_t isCA)
+= let extValue_payload: x509_basicConstraints_extValue_payload_t isCA = ((isCA <: asn1_boolean_true_t), pathLen) in
+  (* Prf *) lemma_serialize_x509_basicConstraints_extValue_payload_size isCA extValue_payload;
+
+  let extValue: x509_basicConstraints_extValue_t isCA = extValue_payload in
+  (* Prf *) lemma_serialize_x509_basicConstraints_extValue_size_exact isCA extValue;
+
+  let ext: x509_basicConstraints_t isCA = x509_get_extension
+                                            (OID_BASIC_CONSTRAINTS)
+                                            (serialize_x509_basicConstraints_extValue isCA)
+                                            (extValue)
+                                            (len_of_x509_basicConstraints_extValue true pathLen)
+                                            (criticality)
+                                            in
+  (* return *) ext
+
+let x509_get_basicConstraints_isNotCA
+  (isCA: bool { isCA == false })
+  (criticality: datatype_of_asn1_type BOOLEAN)
+: Tot (x509_basicConstraints_t isCA)
+= let extValue_payload: x509_basicConstraints_extValue_payload_t isCA = isCA <: asn1_boolean_false_t in
+  (* Prf *) lemma_serialize_x509_basicConstraints_extValue_payload_size isCA extValue_payload;
+
+  let extValue: x509_basicConstraints_extValue_t isCA = extValue_payload in
+  (* Prf *) lemma_serialize_x509_basicConstraints_extValue_size_exact isCA extValue;
+
+  let ext: x509_basicConstraints_t isCA = x509_get_extension
+                                            (OID_BASIC_CONSTRAINTS)
+                                            (serialize_x509_basicConstraints_extValue isCA)
+                                            (extValue)
+                                            (len_of_x509_basicConstraints_extValue isCA)
+                                            (criticality)
+                                            in
+  (* return *) ext
+
+(* FIXME: Does not type check for some reason *)
+(*
+let x509_get_basicConstraints
+  (isCA: bool)
+  (criticality: datatype_of_asn1_type BOOLEAN)
+: Tot (
+  if isCA then
+  ( datatype_of_asn1_type INTEGER -> Tot (x509_basicConstraints_t isCA) )
+  else
+  ( x509_basicConstraints_t isCA )
+)
+= if isCA then
+  ( x509_get_basicConstraints_isCA isCA criticality )
+  else
+  ( x509_get_basicConstraints_isNotCA criticality )
