src/riot/x509/X509.ExtFields.ExtendedKeyUsage.Tests.fst
@@ -1,5 +1,5 @@
 module X509.ExtFields.ExtendedKeyUsage.Tests
-(*)
+
 open LowParse.Spec.Base
 open LowParse.Spec.Combinators
 
@@ -16,11 +16,18 @@ module P = FStar.Pervasives
 
 open X509.ExtFields.ExtendedKeyUsage
 
-noextract unfold inline_for_extraction
-let oids: l: list (datatype_of_asn1_type OID) { valid_keyPurposeIDs l }
+#set-options "--z3rlimit 32 --fuel 4 --ifuel 0"
+
+noextract inline_for_extraction
+let oids
+: l: keyPurposeIDs_oids_t
+     { valid_x509_ext_key_usage_ingredients l }
 = [@inline_let] let l = [OID_AT_CN; OID_AT_COUNTRY; OID_AT_ORGANIZATION] in
   assert_norm (valid_keyPurposeIDs l);
+  lemma_serialize_x509_keyPurposeIDs_size l;
   l
+
+#set-options "--fuel 0"
 
 // noextract
 // let norm_kp () : Tac unit = norm [delta_only [
@@ -34,26 +41,37 @@ let oids: l: list (datatype_of_asn1_type OID) { valid_keyPurposeIDs l }
 //   `%FStar.List.Tot.Base.hd;
 // ]; primops; zeta; iota]; trefl ()
 
+
+[@@T.postprocess_with (postprocess_x509_keyPurposeIDs (`%oids))]
+let ty = x509_keyPurposeIDs_t oids
+
 let tm: ty = ((OID_AT_CN, OID_AT_COUNTRY), OID_AT_ORGANIZATION)
 
 let p = parse_x509_keyPurposeIDs oids
 
 let s = serialize_x509_keyPurposeIDs oids
 
-let lemma_serialize_x509_keyPurposeIDs_unfold_test ()
-: Lemma (
- s `serialize` tm ==
- (serialize_asn1_oid_TLV_of OID_AT_CN `serialize` (fst (fst tm)))
-  `Seq.append`
- (serialize_asn1_oid_TLV_of OID_AT_COUNTRY `serialize` (snd (fst tm)))
-  `Seq.append`
- (serialize_asn1_oid_TLV_of OID_AT_ORGANIZATION `serialize` (snd tm))
-)
-= //P.norm_spec (norm_steps_x509_keyPurposeIDs (`%oids)) (serialize_x509_keyPurposeIDs_unfold_spec oids tm);
-  lemma_serialize_x509_keyPurposeIDs_unfold_norm oids tm;
-  lemma_serialize_x509_keyPurposeIDs_unfold oids tm
+// let lemma_serialize_x509_keyPurposeIDs_unfold_test ()
+// : Lemma (
+//  s `serialize` tm ==
+//  (serialize_asn1_oid_TLV_of OID_AT_CN `serialize` (fst (fst tm)))
+//   `Seq.append`
+//  (serialize_asn1_oid_TLV_of OID_AT_COUNTRY `serialize` (snd (fst tm)))
+//   `Seq.append`
+//  (serialize_asn1_oid_TLV_of OID_AT_ORGANIZATION `serialize` (snd tm))
+// )
+// = //P.norm_spec (norm_steps_x509_keyPurposeIDs (`%oids)) (serialize_x509_keyPurposeIDs_unfold_spec oids tm);
+//   lemma_x509_keyPurposeIDs_unique oids;
+//   lemma_serialize_x509_keyPurposeIDs_unfold_norm oids;
+//   lemma_serialize_x509_keyPurposeIDs_unfold oids
 
-#push-options "--z3rlimit 32 --fuel 4 --ifuel 0"
+
+[@@T.postprocess_with (postprocess_x509_keyPurposeIDs (`%oids))]
+let y = len_of_x509_keyPurposeIDs oids
+
+let z = normalize_term y
+
+#push-options "--z3rlimit 256 --fuel 0 --ifuel 0"
 // [@@T.postprocess_with (postprocess_x509_keyPurposeIDs (`%oids))]
 let lemma_serialize_x509_keyPurposeIDs_size_test ()
 : Lemma (
@@ -61,14 +79,27 @@ let lemma_serialize_x509_keyPurposeIDs_size_test ()
   //          P.norm      (norm_steps_x509_keyPurposeIDs (`%oids)) (x509_keyPurposeIDs_t oids) in
   // let tm: ty = ((OID_AT_CN, OID_AT_COUNTRY), OID_AT_ORGANIZATION) in
  // length_of_opaque_serialization s tm < 100
- serialize_x509_keyPurposeIDs_size_spec oids tm < 100
+ // serialize_x509_keyPurposeIDs_size_spec oids < 100
+ // P.norm
+ //   (norm_steps_x509_keyPurposeIDs (`%oids))
+   (length_of_x509_keyPurposeIDs oids) < 100
 )
-= //admit();
+=
+  (* FIXME: Don't know why but this lemma is not working. *)
+  // lemma_length_of_x509_keyPurposeIDs_norm oids;
+  P.norm_spec
+   (norm_steps_x509_keyPurposeIDs (`%oids))
+   (length_of_x509_keyPurposeIDs oids)
+(*)
+;
+
+//admit();
   // let ty = (x509_keyPurposeIDs_t oids) in
   // let tm: ty = ((OID_AT_CN, OID_AT_COUNTRY), OID_AT_ORGANIZATION) in
   //P.norm_spec (norm_steps_x509_keyPurposeIDs (`%oids)) (serialize_x509_keyPurposeIDs_unfold_spec oids tm);
-  // lemma_serialize_x509_keyPurposeIDs_size_norm oids tm;
-  lemma_serialize_x509_keyPurposeIDs_size oids tm
+  // lemma_serialize_x509_keyPurposeIDs_size_norm oids;
+  // lemma_serialize_x509_keyPurposeIDs_size oids
+  lemma_length_of_x509_keyPurposeIDs_norm oids
   // lemma_serialize_asn1_oid_TLV_of_size OID_AT_CN OID_AT_CN;
   // lemma_serialize_asn1_oid_TLV_of_size OID_AT_COUNTRY OID_AT_COUNTRY;
   // lemma_serialize_asn1_oid_TLV_of_size OID_AT_ORGANIZATION OID_AT_ORGANIZATION
