src/test/RIoT.Test.Definitions.fst
@@ -29,7 +29,7 @@ open RIoT.Base
 
 module Ed25519 = Hacl.Ed25519
 
-#set-options "--z3rlimit 32 --fuel 0 --ifuel 0"
+#set-options "--z3rlimit 64 --fuel 0 --ifuel 0"
 
 let aliasKeyCrt_version: x509_version_t = x509_version_3
 let aliasKeyCrt_serialNumber: x509_serialNumber_t
@@ -43,13 +43,13 @@ let s_common: x509_RDN_x520_attribute_string_t COMMON_NAME IA5_STRING
 let s_org: x509_RDN_x520_attribute_string_t ORGANIZATION IA5_STRING
 = asn1_get_character_string #IA5_STRING 2ul (B32.create 2ul 0uy)
 
-#push-options "--z3rlimit 64"
 let s_country: x509_RDN_x520_attribute_string_t COMMON_NAME PRINTABLE_STRING
 = asn1_get_character_string #PRINTABLE_STRING 2ul (B32.create 2ul 0x41uy)
-#pop-options
 
 let notBefore: datatype_of_asn1_type Generalized_Time
 = B32.create 13ul 0uy
 let notAfter: datatype_of_asn1_type Generalized_Time
 = B32.create 13ul 0uy
 
+let aliasKeyCrt_keyID: datatype_of_asn1_type OCTET_STRING
+= (|1ul, B32.create 1ul 1uy|)
